refactor: Change `Scale.notes` to `Scale.pitches`

Prismriver/Repr/Pitch.lean
@@ -1,9 +1,11 @@
 namespace Prismriver
 
-/-- A set of permitted notes -/
+/-- A set of permitted pitches -/
 class PseudoScale (P : Type) where
   name : String
-  -- The list of all permitted notes on the scale. For periodic scales this should return empty
+  isFinite : Bool := false
+  /-- The list of all permitted notes on the scale. For periodic and infinite
+  scales this should return empty -/
   allNotes : List P := []
 
 /-- We make no distinction between scales and tuning systems. They are
@@ -15,8 +17,8 @@ class PseudoScaleLift (P₁ P₂ : Type) (src : PseudoScale P₁) (dst : PseudoS
 
 /-- A scale with a repeating fundamental interval -/
 class Scale (P : Type) extends PseudoScale P where
-  -- List all notes in the n₀th interval (usually an octave)
-  notes (n₀ : Int) : List P
+  /-- List all notes in the n₀th interval (usually an octave) -/
+  pitches (n₀ : Int) : List P
 
 class ScaleLift (P₁ P₂ : Type) (src : Scale P₁) (dst : Scale P₂)
   extends PseudoScaleLift P₁ P₂ src.toPseudoScale dst.toPseudoScale where
@@ -29,10 +31,10 @@ structure Pitch where
 
 instance scale : Scale Pitch where
   name := "12-ET"
-  notes octave := List.finRange 12 |>.map λ offset =>
+  pitches octave := List.finRange 12 |>.map λ offset =>
     { octave, offset }
 
-theorem et12_notes (octave : Int) : (scale.notes octave).length = 12 := by
+theorem et12_notes (octave : Int) : (scale.pitches octave).length = 12 := by
   rfl
 
 end ET12
